SporkProofs/Preservation.lean
@@ -4,19 +4,19 @@ import SporkProofs.WFSyntax
 import SporkProofs.WFSemantics
 
 namespace Step
-  theorem preserve_retjoin_stack_cons
+  theorem preserve_exitsig_stack_cons
     {P K f ρ₁ ρ₂ X₁ X₂ c₁ c₂}
     (req : P[f]!.B[c₁]!.r = P[f]!.B[c₂]!.r) :
-      CallStack.retjoin P (K ⬝ ⟨f, ρ₁, X₁, c₁⟩) =
-      CallStack.retjoin P (K ⬝ ⟨f, ρ₂, X₂, c₂⟩)
+      CallStack.exitsig P (K ⬝ ⟨f, ρ₁, X₁, c₁⟩) =
+      CallStack.exitsig P (K ⬝ ⟨f, ρ₂, X₂, c₂⟩)
     := by simp at req; cases K <;> simp[req]
 
-  @[simp] theorem preserve_retjoin_stack_cons_cons {P K k k'} :
-      (K ⬝ k ⬝ k').retjoin P = (K ⬝ k).retjoin P :=
+  @[simp] theorem preserve_exitsig_stack_cons_cons {P K k k'} :
+      (K ⬝ k ⬝ k').exitsig P = (K ⬝ k).exitsig P :=
     by cases K <;> rfl
 
-  @[simp] theorem preserve_retjoin_stack_cons_nonnil {P K k} :
-      K ≠ ∅ → (K ⬝ k).retjoin P = K.retjoin P := by
+  @[simp] theorem preserve_exitsig_stack_cons_nonnil {P K k} :
+      K ≠ ∅ → (K ⬝ k).exitsig P = K.exitsig P := by
     cases K <;> intro nn
     · case nil => contradiction
     · case cons => rfl
@@ -25,95 +25,95 @@ namespace Step
     | s, .nil, h => h
     | s, K ⬝ k, h => by simp
 
-  @[simp] theorem preserve_retjoin_stack_append {P K k} : {K' : CallStack} ->
-      CallStack.retjoin P (K ⬝ k ++ K') = CallStack.retjoin P (K ⬝ k)
+  @[simp] theorem preserve_exitsig_stack_append {P K k} : {K' : CallStack} ->
+      CallStack.exitsig P (K ⬝ k ++ K') = CallStack.exitsig P (K ⬝ k)
     | .nil => rfl
-    | K' ⬝ k' => preserve_retjoin_stack_cons_nonnil
+    | K' ⬝ k' => preserve_exitsig_stack_cons_nonnil
                    (stack_append_left_nonnil (K ⬝ k) K' (by simp)) ▸
-                 preserve_retjoin_stack_append (K' := K')
+                 preserve_exitsig_stack_append (K' := K')
 
-  theorem preserve_retjoin {P : Program} : {R R' : ThreadTree} ->
+  theorem preserve_exitsig {P : Program} : {R R' : ThreadTree} ->
                          P ⊢ R ↦ R' -> P ⊢ R WF-tree ->
-                         R.retjoin P = R'.retjoin P
+                         R.exitsig P = R'.exitsig P
   | R, R', s => by
     cases s <;> intro Rwf
     · case congr_parent Rp Rp' Rc s =>
-        simp only [ThreadTree.retjoin]; match Rwf with
-          | .node Rpwf Rcwf Rpp Rcp => exact preserve_retjoin s Rpwf
+        simp only [ThreadTree.exitsig]; match Rwf with
+          | .node Rpwf Rcwf Rpp Rcp => exact preserve_exitsig s Rpwf
     · case congr_child Rp Rc Rc' s =>
         rfl
     · case stmt f K ρ X b e v c a =>
-      apply preserve_retjoin_stack_cons
+      apply preserve_exitsig_stack_cons
       rfl
     · case goto f K ρ X b bnext =>
-      apply preserve_retjoin_stack_cons
-      let flt : f < P.size := Rwf.get.K.current.flt
-      let x := congrArg (·.2) Rwf.get.c.goto_bnext.bsig
+      apply preserve_exitsig_stack_cons
+      have flt : f < P.size := Rwf.get.K.current.flt
+      have x := congrArg (·.2) Rwf.get.c.goto_bnext.bsig
       simp at x
       rw[getElem!_pos P f flt,
          getElem!_pos P[f].B bnext.b Rwf.get.c.goto_bnext.blt,
-         getElem!_pos P[f].B b (let y := Rwf.get.K.current.blt
-                                by simp at y; rw[List.length_map]; exact y)]
+         getElem!_pos P[f].B b (by have y := Rwf.get.K.current.blt
+                                   simp at y; rw[List.length_map]; exact y)]
       simp; exact x.symm
     · case ite_true f K ρ X b cond bthen belse n a neq0 =>
-      apply preserve_retjoin_stack_cons
-      let flt := Rwf.get.K.current.flt
+      apply preserve_exitsig_stack_cons
+      have flt := Rwf.get.K.current.flt
       rw[getElem!_pos P f flt]
       rw[getElem!_pos P[f].B bthen.b Rwf.get.c.ite_bthen.blt]
-      rw[getElem!_pos P[f].B b (let y := Rwf.get.K.current.blt
-                                by simp at y; rw[List.length_map]; exact y)]
+      rw[getElem!_pos P[f].B b (by have y := Rwf.get.K.current.blt
+                                   simp at y; rw[List.length_map]; exact y)]
       exact congrArg (·.2) Rwf.get.c.ite_bthen.bsig.symm
     · case ite_false f K ρ X b cond bthen belse a =>
-      apply preserve_retjoin_stack_cons
-      let flt := Rwf.get.K.current.flt
+      apply preserve_exitsig_stack_cons
+      have flt := Rwf.get.K.current.flt
       rw[getElem!_pos P f flt]
       rw[getElem!_pos P[f].B belse.b Rwf.get.c.ite_belse.blt]
-      rw[getElem!_pos P[f].B b (let y := Rwf.get.K.current.blt
-                                by simp at y; rw[List.length_map]; exact y)]
+      rw[getElem!_pos P[f].B b (by have y := Rwf.get.K.current.blt
+                                   simp at y; rw[List.length_map]; exact y)]
       exact congrArg (·.2) Rwf.get.c.ite_belse.bsig.symm
     · case call f g K ρ b X x bret =>
-      apply preserve_retjoin_stack_cons
-      let flt := Rwf.get.K.current.flt
+      apply preserve_exitsig_stack_cons
+      have flt := Rwf.get.K.current.flt
       rw[getElem!_pos P f flt]
       rw[getElem!_pos P[f].B bret.b Rwf.get.c.call_bret.blt]
-      rw[getElem!_pos P[f].B b (let y := Rwf.get.K.current.blt
-                                by simp at y; rw[List.length_map]; exact y)]
+      rw[getElem!_pos P[f].B b (by have y := Rwf.get.K.current.blt
+                                   simp at y; rw[List.length_map]; exact y)]
       exact congrArg (·.2) Rwf.get.c.call_bret.bsig.symm
     · case retn f g K ρ X Y y b bret =>
-      apply preserve_retjoin_stack_cons (K := K)
+      apply preserve_exitsig_stack_cons (K := K)
       simp
     · case spork f K ρ X b bbody bspwn =>
-      apply preserve_retjoin_stack_cons
-      let flt := Rwf.get.K.current.flt
+      apply preserve_exitsig_stack_cons
+      have flt := Rwf.get.K.current.flt
       rw[getElem!_pos P f flt]
       rw[getElem!_pos P[f].B bbody.b Rwf.get.c.spork_bbody.blt]
-      rw[getElem!_pos P[f].B b (let y := Rwf.get.K.current.blt
-                                by simp at y; rw[List.length_map]; exact y)]
+      rw[getElem!_pos P[f].B b (by have y := Rwf.get.K.current.blt
+                                   simp at y; rw[List.length_map]; exact y)]
       exact congrArg (·.2) Rwf.get.c.spork_bbody.bsig.symm
     · case promote f unpr bspwn prom X K b K' C u p =>
-      let flt := Rwf.get.K.current.flt
+      have flt := Rwf.get.K.current.flt
       simp
-      apply preserve_retjoin_stack_cons
+      apply preserve_exitsig_stack_cons
       simp
     · case spoin_unpr f K ρ bspwn X b bunpr bprom =>
-      apply preserve_retjoin_stack_cons
-      let flt := Rwf.get.K.current.flt
+      apply preserve_exitsig_stack_cons
+      have flt := Rwf.get.K.current.flt
       rw[getElem!_pos P f flt]
       rw[getElem!_pos P[f].B bunpr.b Rwf.get.c.spoin_bunpr.blt]
-      rw[getElem!_pos P[f].B b (let y := Rwf.get.K.current.blt
-                                by simp at y; rw[List.length_map]; exact y)]
+      rw[getElem!_pos P[f].B b (by have y := Rwf.get.K.current.blt
+                                   simp at y; rw[List.length_map]; exact y)]
       exact congrArg (·.2) Rwf.get.c.spoin_bunpr.bsig.symm
     · case spoin_prom f g K ρ X b b' bunpr bprom Y y bspwn u =>
-      apply preserve_retjoin_stack_cons
-      let flt := Rwf.parent.get.K.current.flt
+      apply preserve_exitsig_stack_cons
+      have flt := Rwf.parent.get.K.current.flt
       rw[getElem!_pos P f flt]
       rw[getElem!_pos P[f].B bprom.b Rwf.parent.get.c.spoin_bprom.blt]
-      rw[getElem!_pos P[f].B b (let y := Rwf.parent.get.K.current.blt
-                                by simp at y; rw[List.length_map]; exact y)]
+      rw[getElem!_pos P[f].B b (by have y := Rwf.parent.get.K.current.blt
+                                   simp at y; rw[List.length_map]; exact y)]
       exact congrArg (·.2) Rwf.parent.get.c.spoin_bprom.bsig.symm
 
     -- · case promote f unpr g prom X K c K' u p =>
-    --     simp; rw[preserve_retjoin_stack_cons]
+    --     simp; rw[preserve_exitsig_stack_cons]
 
   theorem preserve_prom {P : Program} : {R R' : ThreadTree} ->
                          P ⊢ R ↦ R' -> P ⊢ R WF-tree -> R.prom = R'.prom
@@ -168,7 +168,7 @@ namespace Step
 
     · case congr_child Rp Rc Rc' Rc_Rc' Rpwf Rcwf Rcp Rpp =>
         exact node Rpwf (preservation Pwf Rcwf Rc_Rc')
-                        (preserve_retjoin Rc_Rc' Rcwf ▸ Rpp)
+                        (preserve_exitsig Rc_Rc' Rcwf ▸ Rpp)
                         (preserve_prom Rc_Rc' Rcwf ▸ Rcp)
 
     · case stmt f K ρ X b e v c a wf =>
@@ -181,19 +181,19 @@ namespace Step
     · case goto f K ρ X b bnext wf =>
         apply (· ⬝wf ·)
         · apply goto!h wf.K.current wf.c!.goto_bnext
-        · let h : P[f]!.B[bnext.b]! = _ := wf.c!.goto_bnext.bsig!
+        · have h : P[f]!.B[bnext.b]! = _ := wf.c!.goto_bnext.bsig!
           simpa only [StackFrame.ret!, getters, h] using wf.K.tail
 
     · case ite_true f K ρ X b cond bthen belse n cond_n neq0 wf =>
         apply (· ⬝wf ·)
         · apply goto!h wf.K.current wf.c!.ite_bthen
-        · let h : P[f]!.B[bthen.b]! = _ := wf.c!.ite_bthen.bsig!
+        · have h : P[f]!.B[bthen.b]! = _ := wf.c!.ite_bthen.bsig!
           simpa only [StackFrame.ret!, getters, h] using wf.K.tail
 
     · case ite_false f K ρ X cond b bthen belse cond_0 wf =>
         apply (· ⬝wf ·)
         · apply goto!h wf.K.current wf.c!.ite_belse
-        · let h : P[f]!.B[belse.b]! = _ := wf.c!.ite_belse.bsig!
+        · have h : P[f]!.B[belse.b]! = _ := wf.c!.ite_belse.bsig!
           simpa only [StackFrame.ret!, getters, h] using wf.K.tail
 
     · case call f g K ρ b X x bret wf =>
@@ -202,15 +202,15 @@ namespace Step
           · rw[getElem!_pos X x wf.c.call_args,
                X.getElem_length wf.c.call_args]
             simpa [← List.getElem_map Func.fsig] using wf.c.call_arity
-        · let p := wf.K.tail
-          let s := congrArg BlockSig.r wf.c!.call_bret.bsig!
+        · have p := wf.K.tail
+          have s := congrArg BlockSig.r wf.c!.call_bret.bsig!
           simp only [StackFrame.ret!, getters, CallStack.bsig!, StackFrame.bsig!] at p s ⊢
           rw[s]
           exact p
         · apply goto_rets!h wf.K.current
-          · let glt : g < P.size := by simpa using wf.c.call_flt
-            let zlt : 0 < P[g].B.length := Pwf⁅g⁆.head.zero_lt_map
-            let gsig : P[g].B[0].r = P[g].fsig.ret :=
+          · have glt : g < P.size := by simpa using wf.c.call_flt
+            have zlt : 0 < P[g].B.length := Pwf⁅g⁆.head.zero_lt_map
+            have gsig : P[g].B[0].r = .retn P[g].fsig.ret :=
               congrArg BlockSig.r Pwf⁅g⁆.head.get0eq_map
             simpa only [getters,
                        CallStack.bsig!,
@@ -224,7 +224,7 @@ namespace Step
             using wf.c!.call_bret
 
     · case retn f g K ρ X Y y b bret wf =>
-        let ypf : (Y[y]'wf.c.retn_args).length = P[g]!.B[b]!.r :=
+        have ypf : (Y[y]'wf.c.retn_args).length = P[g]!.B[b]!.r.n :=
           Y.getElem_length wf.c.retn_args ▸
           wf.c.retn_length ▸
           getElem!_pos P g wf.K.current.flt ▸
@@ -244,13 +244,13 @@ namespace Step
         apply (· ⬝wf ·)
         · apply StackFrame.WF.mk
           · apply And.intro
-            · let apf := congrArg BlockSig.Γ wf.c.spork_bbody.bsig
+            · have apf := congrArg BlockSig.Γ wf.c.spork_bbody.bsig
               simp only [getters] at apf
               rw[getElem!_pos X bbody.args wf.c.spork_bbody.args,
                  X.getElem_length wf.c.spork_bbody.args,
                  ← apf, Option.getD_none, Nat.add_zero]
               exact Nat.le_refl ((P[f]'wf.K.current.flt).B[bbody.b]'wf.c.spork_bbody.blt).Γ
-            · let bpf := congrArg BlockSig.σ wf.c.spork_bbody.bsig
+            · have bpf := congrArg BlockSig.σ wf.c.spork_bbody.bsig
               simp only [getters, CallStack.bsig, StackFrame.bsig] at bpf
               rw[SpawnDeque.pushsig, bpf]
               simp only [getters]
@@ -261,7 +261,7 @@ namespace Step
                 exact congrArg BlockSig.Γ wf.c.spork_bspwn.2
               · exact congrArg BlockSig.σ wf.c.spork_bspwn.2
               · exact wf.c.spork_bspwn.1
-        · let h : P[f]!.B[bbody.b]! = _ := wf.c!.spork_bbody.bsig!
+        · have h : P[f]!.B[bbody.b]! = _ := wf.c!.spork_bbody.bsig!
           simpa only [StackFrame.ret!, getters, h] using wf.K.tail
 
     · case promote f unpr bspwn prom X K b K' c u p wf =>
@@ -275,31 +275,31 @@ namespace Step
         apply (· ⬝wf ·)
         · apply StackFrame.WF.mk
           · apply And.intro
-            · let apf := congrArg BlockSig.Γ wf.c.spoin_bunpr.bsig
+            · have apf := congrArg BlockSig.Γ wf.c.spoin_bunpr.bsig
               simp only [getters] at apf
               rw[getElem!_pos X bunpr.args wf.c.spoin_bunpr.args,
                  X.getElem_length wf.c.spoin_bunpr.args,
                  ← apf, Option.getD_none, Nat.add_zero]
               exact Nat.le_refl ((P[f]'wf.K.current.flt).B[bunpr.b]'wf.c.spoin_bunpr.blt).Γ
-            · let bpf := congrArg BlockSig.σ wf.c.spoin_bunpr.bsig
+            · have bpf := congrArg BlockSig.σ wf.c.spoin_bunpr.bsig
               simp only [getters, CallStack.bsig, StackFrame.bsig,
                          SpawnDeque.pushsig, List.tail_cons] at bpf
               rw[bpf]
           · exact wf.K.current.ρwf.unpush
-        · let h : P[f]!.B[bunpr.b]! = _ := wf.c!.spoin_bunpr.bsig!
+        · have h : P[f]!.B[bunpr.b]! = _ := wf.c!.spoin_bunpr.bsig!
           simpa only [StackFrame.ret!, getters, h] using wf.K.tail
 
     · case spoin_prom f g K ρ X b b' bunpr bprom Y y bspwn K_unpr_nil Rpwf Rcwf ret_prom_nil heq =>
-        let flt : f < P.size := Rpwf.get.K.current.flt
-        let glt : g < P.size := Rcwf.get.K.current.flt
+        have flt : f < P.size := Rpwf.get.K.current.flt
+        have glt : g < P.size := Rcwf.get.K.current.flt
         apply (· ⬝wf ·)
         · apply StackFrame.WF.mk
           · apply And.intro
-            · let apf := congrArg BlockSig.Γ Rpwf.get.c.spoin_bprom.bsig
+            · have apf := congrArg BlockSig.Γ Rpwf.get.c.spoin_bprom.bsig
               simp only [getters, CallStack.bsig, StackFrame.bsig] at apf
               simp only [getters, ThreadTree.promsig,
                          Thread.promsig, CallStack.promsig, SpawnDeque.promsig,
-                         ThreadTree.retjoin, Thread.retjoin, CallStack.retjoin] at heq
+                         ThreadTree.exitsig, Thread.exitsig, CallStack.exitsig] at heq
               rw[List.map_cons, List.cons_append, List.head?_cons, Option.some_inj,
                  getElem!_pos P f flt, getElem!_pos P g glt,
                  getElem!_pos P[g].B b'] at heq
@@ -310,18 +310,18 @@ namespace Step
                  Y.getElem_length Rcwf.get.c.retn_args,
                  Option.getD_none, Nat.add_zero, apf]
               simp only [SpawnDeque.sig, getters, SpawnDeque.out, List.reverseAux, List.map, List.head]
-              let bpf := Rcwf.get.c.retn_length
+              have bpf := Rcwf.get.c.retn_length
               simp only [getters, CallStack.head, CallStack.bsig, StackFrame.bsig] at bpf
               rw[← bpf, ← heq]
               exact Nat.le_refl _
-            · let bpf := congrArg BlockSig.σ Rpwf.get.c.spoin_bprom.bsig
+            · have bpf := congrArg BlockSig.σ Rpwf.get.c.spoin_bprom.bsig
               simp only [getters, CallStack.bsig, StackFrame.bsig,
                          SpawnDeque.pushsig, List.tail_cons] at bpf
               rw[bpf]
               simp[Rpwf.get.K.current.bsig.2]
-          · let a : P[f].B; K.allPromoted ⊢ ⟨[], bspwn :: ρ⟩ WF-deque :=
+          · have a : P[f].B; K.allPromoted ⊢ ⟨[], bspwn :: ρ⟩ WF-deque :=
               Rpwf.get.K.current.ρwf
             exact ⟨a.1, by simp[K_unpr_nil]; exact rfl⟩
-        · let h : P[f]!.B[bprom.b]! = _ := Rpwf.get.c!.spoin_bprom.bsig!
+        · have h : P[f]!.B[bprom.b]! = _ := Rpwf.get.c!.spoin_bprom.bsig!
           simpa only [StackFrame.ret!, getters, h] using Rpwf.get.K.tail
 end Step
